Proofs for basic invariants

Graphlib/DFS-2.lean
@@ -19,8 +19,26 @@ variable (G : WeightedDiGraph V E)
 structure dfs_state [FinEnum V] [DecidableEq E] [DecidableEq V]
     (g: WeightedDiGraph V E) where
     visited : Finset V
+    pathOrder : visited → Nat 
     mother : visited → V
     stack : List V
+
+
+abbrev dfs_invar_stack_is_visited [FinEnum V] [DecidableEq E] [DecidableEq V]
+    (g: WeightedDiGraph V E) (s : dfs_state g):=
+      ∀ x : V, x ∈ s.stack → x ∈ s.visited
+
+abbrev dfs_invar_mother_is_visited [FinEnum V] [DecidableEq E] [DecidableEq V]
+    (g: WeightedDiGraph V E) (s : dfs_state g):=
+      ∀ x : s.visited, s.mother x ∈ s.visited
+
+
+abbrev dfs_invar_mother_decreasing_path_order [FinEnum V] [DecidableEq E] [DecidableEq V]
+    (g: WeightedDiGraph V E) (start : V) (s : dfs_state g)
+    (mother_invar : dfs_invar_mother_is_visited g s)
+    :=
+      ∀ x : s.visited, ↑x ≠ start →
+        s.pathOrder ⟨(s.mother x), by simp_all only [Subtype.forall]⟩  < s.pathOrder x 
 
 
 def dfs_step_expand[FinEnum V] [DecidableEq E] [DecidableEq V]
@@ -46,8 +64,78 @@ def dfs_step_expand[FinEnum V] [DecidableEq E] [DecidableEq V]
         if h: (v ∈ priorState.visited) then priorState.mother ⟨ v, by exact h⟩
         else stackHead
 
-      dfs_state.mk new_visited new_mother new_stack
+      let new_order : new_visited → Nat := fun ⟨v, hv⟩  =>
+        if h: (v ∈ priorState.visited) then priorState.pathOrder ⟨ v, by exact h⟩
+        else priorState.stack.length
 
+      dfs_state.mk new_visited new_order new_mother new_stack
+
+
+lemma dfs_expand_newly_added_are_adjacent --[FinEnum V] [DecidableEq E] [DecidableEq V]
+    (g: WeightedDiGraph V E)
+    (priorState : dfs_state g)
+    (stackHead : V)
+    (stackTail : List V):
+    ∀ x : V, x ∉ priorState.visited ∧ x ∉ stackTail ∧
+      x ∈ (dfs_step_expand g priorState stackHead stackTail).stack →  
+      g.Adj stackHead x := by
+    intro x
+    intro ⟨x_not_visi, ⟨ x_not_on_stack_before, x_on_stack_after ⟩  ⟩
+    unfold dfs_step_expand at x_on_stack_after
+    simp_all
+
+
+lemma dfs_expand_keeps_stack_in_visited --[FinEnum V] [DecidableEq E] [DecidableEq V]
+    (g: WeightedDiGraph V E)
+    (priorState : dfs_state g)
+    (stackHead : V)
+    (stackTail : List V):
+    dfs_invar_stack_is_visited g priorState ∧
+      stackHead ∈ priorState.visited ∧ (∀ x : V, x ∉ priorState.visited → x ∉ stackTail) →
+      dfs_invar_stack_is_visited g (dfs_step_expand g priorState stackHead stackTail) := by
+      intro ⟨ stack_is_visited_prior, stackhead_visited, x_not_in_stack_tail⟩ 
+      unfold dfs_invar_stack_is_visited
+      intro x 
+      intro x_now_on_stack
+      unfold dfs_step_expand
+      simp_all
+      by_cases x_was_visited : x ∈ priorState.visited
+      · left
+        exact x_was_visited
+      · right
+        apply And.intro
+        · apply (dfs_expand_newly_added_are_adjacent g priorState stackHead stackTail)
+          simp_all
+        · exact x_was_visited
+
+
+lemma dfs_expand_keeps_mother_in_visited --[FinEnum V] [DecidableEq E] [DecidableEq V]
+    (g: WeightedDiGraph V E)
+    (priorState : dfs_state g)
+    (stackHead : V)
+    (stackTail : List V):
+    dfs_invar_mother_is_visited g priorState ∧ stackHead ∈ priorState.visited → dfs_invar_mother_is_visited g (dfs_step_expand g priorState stackHead stackTail) := by
+      intro mother_is_visited_prior
+      unfold dfs_invar_mother_is_visited
+      intro x
+      simp_all
+      unfold dfs_step_expand
+      simp_all
+      by_cases x_is_already_visited : ↑x ∈ priorState.visited
+      all_goals
+        simp_all
+
+
+--abbrev [FinEnum V] [DecidableEq E] [DecidableEq V]
+--    (g: WeightedDiGraph V E) (start : V) (s : dfs_state g start):=
+--      ∀ x : s.visited, (∃ y ∈ s.stack, y.node = x) ∨ ∀ y : V, (g.Adj x y) → y ∈ s.visited
+
+
+
+
+
+
+---------------------------------------------------------------------------------------
 
 def dfs_step [FinEnum V] [DecidableEq E] [DecidableEq V]
     (g: WeightedDiGraph V E) (goal : V)
@@ -59,6 +147,50 @@ def dfs_step [FinEnum V] [DecidableEq E] [DecidableEq V]
     if h : s = goal then (priorState, some (some s))
     else
       (dfs_step_expand g priorState s xs, none)
+
+
+lemma dfs_step_keeps_stack_in_visited --[FinEnum V] [DecidableEq E] [DecidableEq V]
+    (g: WeightedDiGraph V E)
+    (priorState : dfs_state g):
+    ∀ goal : V,
+    dfs_invar_stack_is_visited g priorState →
+      dfs_invar_stack_is_visited g (dfs_step g goal priorState).fst := by
+        intro goal
+        intro stack_is_visited_prior 
+        unfold dfs_step
+        split
+        · simp_all
+          exact stack_is_visited_prior
+        next _ head tail head_tail_compose =>
+        split
+        · simp_all
+          exact stack_is_visited_prior
+        apply dfs_expand_keeps_stack_in_visited
+        simp_all
+        constructor
+        · exact stack_is_visited_prior
+        intro y y_not_visited
+        intro y_in_tail
+        simp_all
+      
+
+
+lemma dfs_step_keeps_mother_in_visited --[FinEnum V] [DecidableEq E] [DecidableEq V]
+    (g: WeightedDiGraph V E)
+    (priorState : dfs_state g):
+    ∀ goal : V,
+    dfs_invar_stack_is_visited g priorState ∧ dfs_invar_mother_is_visited g priorState →
+      dfs_invar_mother_is_visited g (dfs_step g goal priorState).fst := by
+      intro goal
+      intro ⟨ mother_is_visited_prior, stack_is_visited_prior ⟩ 
+      unfold dfs_step
+      split
+      · simp_all
+      next _ head tail head_tail_compose =>
+      split
+      · simp_all
+      apply dfs_expand_keeps_mother_in_visited
+      simp_all
 
 
 
@@ -81,9 +213,10 @@ def dfs[ FinEnum V] [DecidableEq E] [DecidableEq V]
     (g: WeightedDiGraph V E) (start : V) (goal : V)
     (priorState : dfs_state g) :
     (Option (Option V)) :=
-  let initialVisited : Finset V := ⟨ {start},  by sorry ⟩ 
+  let initialVisited : Finset V := ⟨ {start},  by simp ⟩ 
   let initialMother : initialVisited → V := fun x => start 
+  let initialPathOrder : initialVisited → Nat := fun x => 0 
   let initialStack : List V := [start]
-  let startState : dfs_state g := dfs_state.mk initialVisited initialMother initialStack
+  let startState : dfs_state g := dfs_state.mk initialVisited initialPathOrder initialMother initialStack
 
   (dfs_recurse g goal startState).2
